## Proposition
For any $n \in \mathbb{N}$, $Fib(n) = \frac {\varphi^n - \psi^n} {\sqrt 5}$.  

## Proof
### Base cases
When $k = 0$, $Fib(0) = 0$  
When $k = 1$, $Fib(1) = 1$  

### Inductive step
Assume that the statement holds for $Fib(k)$ and $Fib(k - 1)$, meaning that   

$Fib(k + 1)$  
$= Fib(k) + Fib(k-1)$  
$= \frac {\varphi^k - \psi^k} {\sqrt 5} + \frac {\varphi^{k-1} - \psi^{k-1}} {\sqrt 5}$  
$= \frac {\varphi^k (\frac {\varphi + 1} \varphi) - \psi^k (\frac {\psi + 1} \psi)} {\sqrt 5}$  

Since $\varphi^2 = \varphi + 1$ and $\psi^2 = \psi + 1$,  

$Fib(k + 1) = \frac {\varphi^{k+1} - \psi^{k+1}} {\sqrt 5}$

---
#### References
[Induction](https://en.wikipedia.org/wiki/Mathematical_induction)